AutoProof: enabled invariant generation. updated array translation.

eve/Src/Delivery/studio/tools/autoproof/arrays.bpl
@@ -40,7 +40,7 @@ procedure ARRAY.make(
 			u: int where is_integer_32(u)
 		);
 	requires l == 1; // pre tag:lower_equals_1
-	requires u >= 0; // pre
+	requires u >= 0; // pre tag:upper_not_negative
 	ensures Heap[c, ARRAY.count] == u;
 	ensures ARRAY.inv(Heap, c);
 	modifies Heap;
@@ -53,7 +53,7 @@ procedure ARRAY.make_filled<alpha>(
 			u: int where is_integer_32(u)
 		);
 	requires l == 1; // pre tag:lower_equals_1
-	requires u >= 0; // pre
+	requires u >= 0; // pre tag:upper_not_negative
 	ensures Heap[c, ARRAY.count] == u;
 	ensures ARRAY.inv(Heap, c);
 	modifies Heap;
@@ -63,23 +63,35 @@ function fun.ARRAY.has<alpha>(h: HeapType, c: ref, val: alpha) returns (bool) {
 	(exists i: int :: (fun.ARRAY.is_index(h, c, i) && (fun.ARRAY.item(h, c, i) == val)))
 }
 
+function fun.ARRAY.occurrences<alpha>(heap: HeapType, a: ref, o: alpha) returns (int) {
+	occ(heap, a, o, heap[a, ARRAY.count])
+}
+
+function occ<alpha>(h: HeapType, a: ref, o: alpha, i: int) returns (int);
+axiom (forall<alpha> h: HeapType, a: ref, o: alpha ::
+			{ occ(h, a, o, 0) }
+		occ(h, a, o, 0) == 0);
+axiom (forall<alpha> h: HeapType, a: ref, o: alpha, i: int ::
+			{ occ(h, a, o, i) }
+		(h[a, area][i] == o) ==> (occ(h, a, o, i) == occ(h, a, o, i-1) + 1));
+axiom (forall<alpha> h: HeapType, a: ref, o: alpha, i: int ::
+			{ occ(h, a, o, i) }
+		(h[a, area][i] != o) ==> (occ(h, a, o, i) == occ(h, a, o, i-1)));
+
 procedure ARRAY.subarray(a: ref, l: int, u: int) returns (result: ref);
-	requires fun.ARRAY.is_index(Heap, a, l);
-	requires (l-1) <= u && u <= fun.ARRAY.count(Heap, a);
-	// requires (forall i_46: int :: (((1) <= (i_46)) && ((i_46) <= ((fun.ARRAY.count(Heap, a)) - (1)))) ==> ((fun.ARRAY.item(Heap, a, i_46)) <= (fun.ARRAY.item(Heap, a, (i_46) + (1)))));
-	// ensures !old(Heap)[result, allocated];
-	// ensures Heap[result, ARRAY.count] == u-l+1;
-	// ensures attached(Heap, result, type_of(a));
-	// modifies Heap;
-	// ensures result != a;
-	// ensures (forall i: int :: {fun.ARRAY.has(Heap, a, i)} {fun.ARRAY.has(Heap, result, i)}fun.ARRAY.has(Heap, a, i) == fun.ARRAY.has(Heap, result, i));
-	// ensures (forall i_46: int :: (((1) <= (i_46)) && ((i_46) <= ((fun.ARRAY.count(Heap, result)) - (1)))) ==> ((fun.ARRAY.item(Heap, result, i_46)) <= (fun.ARRAY.item(Heap, result, (i_46) + (1)))));
-	// ensures (forall i: int :: (1 <= i && i <= (u-l+1)) ==> (fun.ARRAY.item(Heap, result, i) == fun.ARRAY.item(Heap, a, l+i-1)));
-  // ensures (forall<beta> o: ref, f: Field beta :: (old(Heap[o, allocated])) ==> (Heap[o, f] == old(Heap[o, f])));
+	requires fun.ARRAY.is_index(Heap, a, l) || fun.ARRAY.is_index(Heap, a, u); // pre tag:lower_or_upper_in_bounds
+	requires (l-1) <= u && u <= fun.ARRAY.count(Heap, a); // pre tag:range_in_bounds
+	ensures !old(Heap)[result, allocated];
+	ensures Heap[result, ARRAY.count] == u-l+1;
+	ensures attached(Heap, result, type_of(a));
+	ensures ARRAY.inv(Heap, result);
+	modifies Heap;
+	ensures (forall i: int :: (1 <= i && i <= (u-l+1)) ==> (fun.ARRAY.item(Heap, result, i) == fun.ARRAY.item(Heap, a, l+i-1)));
+	ensures (forall<beta> o: ref, f: Field beta :: (old(Heap[o, allocated])) ==> (Heap[o, f] == old(Heap[o, f])));
 
 // Array invariants
 function ARRAY.inv(h: HeapType, a: ref) returns (bool) {
-	(a != Void) ==> (h[a, ARRAY.count] >= 0)
+	(a != Void) ==> (h[a, ARRAY.count] >= 0 && is_integer_32(h[a, ARRAY.count]))
 }
 function ARRAY#ref#.inv(h: HeapType, a: ref, ct: Type) returns (bool) {
 	ARRAY.inv(h, a) &&
@@ -92,108 +104,3 @@ function ARRAY#int#.inv(h: HeapType, a: ref) returns (bool) {
 function ARRAY#bool#.inv(h: HeapType, a: ref) returns (bool) {
 	ARRAY.inv(h, a)
 }
-
-// procedure ARRAY#int#.make(
-			// c: ref where attached(Heap, c, ARRAY#int#),
-			// l: int where is_integer_32(l),
-			// u: int where is_integer_32(u)
-		// );
-	// requires l <= u + 1; // pre line:1
-	// ensures Heap[c, ARRAY.lower] == l;
-	// ensures Heap[c, ARRAY.upper] == u;
-	// ensures ARRAY.$inv(Heap, c);
-	// ensures (forall i: int :: ARRAY.$is_index(Heap, c, i) ==> ARRAY.$item(Heap, c, i) == 0);
-	// modifies Heap;
-	// ensures (forall<beta> o: ref, f: Field beta :: (o != c || (f != ARRAY.lower && f != ARRAY.upper && f != ARRAY.count && f != $area)) ==> (Heap[o, f] == old(Heap)[o, f]));
-
-// procedure ARRAY#int#.make_filled(
-			// c: ref where attached(Heap, c, ARRAY#int#),
-			// l: int where is_integer_32(l),
-			// u: int where is_integer_32(u),
-			// v: int where is_integer_32(v)
-		// );
-	// requires l <= u + 1;
-	// ensures Heap[c, ARRAY.lower] == l;
-	// ensures Heap[c, ARRAY.upper] == u;
-	// ensures ARRAY.$inv(Heap, c);
-	// ensures (forall i: int :: ARRAY.$is_index(Heap, c, i) ==> ARRAY.$item(Heap, c, i) == v);
-	// modifies Heap;
-	// ensures (forall<beta> o: ref, f: Field beta :: (o != c) ==> (Heap[o, f] == old(Heap)[o, f]));
-
-// procedure ARRAY#int#.put(
-			// c: ref where attached(Heap, c, ARRAY#int#),
-			// item: int where is_integer_32(item),
-			// pos: int where is_integer_32(pos)
-		// );
-	// requires ARRAY.$is_index(Heap, c, pos); // pre line:1
-	// ensures ARRAY.$item(Heap, c, pos) == item;
-	// ensures ARRAY.$inv(Heap, c);
-	// modifies Heap;
-	// ensures (forall<beta> o: ref, f: Field beta :: (o != c || f != $area) ==> (Heap[o, f] == old(Heap)[o, f]));
-	// ensures (forall i: int :: (ARRAY.$is_index(Heap, c, i) && i != pos) ==> ARRAY.$item(Heap, c, i) == old(ARRAY.$item(Heap, c, i)));
-
-// procedure ARRAY#int#.item(
-			// c: ref where attached(Heap, c, ARRAY#int#),
-			// pos: int where is_integer_32(pos)
-		// ) returns (result: int);
-	// requires ARRAY.$is_index(Heap, c, pos); // pre line:1
-	// ensures result == ARRAY.$item(Heap, c, pos);
-
-// procedure ARRAY#int#.count(
-			// c: ref where attached(Heap, c, ARRAY#int#)
-		// ) returns (result: int);
-	// ensures result == Heap[c, ARRAY.count];
-
-// function fun.ARRAY#int#.count(heap: HeapType, c: ref) returns (int) {
-	// heap[c, ARRAY.count]
-// }
-
-// procedure ARRAY#int#.has(
-			// c: ref where attached(Heap, c, ARRAY#int#),
-			// val: int where is_integer_32(val)
-		// ) returns (result: bool);
-	// ensures result == (exists i: int :: (ARRAY.$is_index(Heap, c, i) && (ARRAY.$item(Heap, c, i) == val)));
-
-// axiom (forall heap: HeapType, c: ref :: (fun.ARRAY#int#.count(heap, c) == 0) ==> (!(exists i: int :: ARRAY.$is_index(heap, c, i))));
-
-// function fun.ARRAY#int#.has(heap: HeapType, c: ref, val: int) returns (bool) {
-	// (exists i: int :: (ARRAY.$is_index(heap, c, i) && (ARRAY.$item(heap, c, i) == val)))
-// }
-
-// function fun.ARRAY#int#.has_not(heap: HeapType, c: ref, val: int) returns (bool) {
-	// (forall i: int :: (ARRAY.$is_index(heap, c, i) ==> !(ARRAY.$item(heap, c, i) == val)))
-// }
-
-
-// procedure ARRAY#int#.subarray(
-			// c: ref where attached(Heap, c, ARRAY^INTEGER_32^),
-			// l: int where is_integer_32(l),
-			// u: int where is_integer_32(u)
-		// ) returns (result: ref);
-	// requires 1 <= l && l <= fun.ARRAY#int#.count(Heap, c) + 1;
-	// requires 0 <= u && u <= fun.ARRAY#int#.count(Heap, c);
-// //	requires (l <= u) || (l == u + 1);
-	// ensures (forall o: ref :: old(Heap)[o, allocated] ==> o != result);
-	// ensures attached(Heap, result, ARRAY^INTEGER_32^);
-	// ensures ARRAY.$inv(Heap, result);
-	// ensures Heap[result, ARRAY.lower] == 1;
-	// ensures Heap[result, ARRAY.count] == (u - l + 1);
-	// ensures 0 <= fun.ARRAY#int#.count(Heap, result) && fun.ARRAY#int#.count(Heap, result) <= fun.ARRAY#int#.count(Heap, c);
-	// ensures (forall i: int :: ARRAY.$is_index(Heap, result, i) ==> ARRAY.$item(Heap, result, i) == ARRAY.$item(Heap, c, i + l - 1));
-	// ensures (forall i: int :: ARRAY.$is_index(Heap, result, i) ==> ARRAY.$item(Heap, result, i) == ARRAY.$item(Heap, c, i + l - 1));
-	// modifies Heap;
-	// ensures (forall<beta> o: ref, f: Field beta :: (o != result) ==> (Heap[o, f] == old(Heap)[o, f]));
-
-
-// procedure ARRAY#ref#.make(
-			// c: ref where attached(Heap, c, ARRAY#ref#),
-			// l: int where is_integer_32(l),
-			// u: int where is_integer_32(u)
-		// );
-	// requires l < u;
-	// ensures Heap[c, ARRAY.lower] == l;
-	// ensures Heap[c, ARRAY.upper] == u;
-	// ensures ARRAY.$inv(Heap, c);
-	// ensures (forall i: int :: ARRAY.$is_index(Heap, c, i) ==> ARRAY.$item(Heap, c, i) == Void);
-	// modifies Heap;
-	// ensures (forall<beta> o: ref, f: Field beta :: (o != c) ==> (Heap[o, f] == old(Heap)[o, f]));
