eve/Src/framework/eiffel2boogie/exec/result/e2b_loop_invariant_violation.e
@@ -1,0 +1,92 @@
+note
+	description: "TODO"
+	date: "$Date$"
+	revision: "$Revision$"
+
+class
+	E2B_LOOP_INVARIANT_VIOLATION
+
+inherit
+	E2B_VERIFICATION_ERROR
+		redefine
+			multi_line_message
+		end
+
+create
+	make
+
+feature -- Status report
+
+	is_on_entry: BOOLEAN
+			-- Is this violation on loop entry?
+
+	is_on_iteration: BOOLEAN
+			-- Is this violation on loop iterations?
+
+feature -- Status setting
+
+	set_on_entry
+			-- Set `is_on_entry'.
+		do
+			is_on_entry := True
+		ensure
+			is_on_entry: is_on_entry
+		end
+
+	set_on_iteration
+			-- Set `is_on_iteration'.
+		do
+			is_on_iteration := True
+		ensure
+			is_on_iteration: is_on_iteration
+		end
+
+feature -- Display
+
+	single_line_message (a_formatter: TEXT_FORMATTER)
+			-- <Precursor>
+		do
+			if is_on_entry then
+				if attached tag then
+					a_formatter.add ("Loop invariant ")
+					a_formatter.add_manifest_string (tag)
+					a_formatter.add (" might not hold on entry.")
+				else
+					a_formatter.add ("Loop invariant might not hold on entry (unnamed assertion).")
+				end
+			else
+				check is_on_iteration end
+				if attached tag then
+					a_formatter.add ("Loop invariant ")
+					a_formatter.add_manifest_string (tag)
+					a_formatter.add (" might not be maintained.")
+				else
+					a_formatter.add ("Loop invariant might not be maintained (unnamed assertion).")
+				end
+			end
+		end
+
+	multi_line_message (a_formatter: TEXT_FORMATTER)
+			-- <Precursor>
+		do
+			if is_on_entry then
+				if attached tag then
+					a_formatter.add ("Loop invariant ")
+					a_formatter.add_manifest_string (tag)
+					a_formatter.add (" might not hold on entry.")
+				else
+					a_formatter.add ("Loop invariant might not hold on entry (unnamed assertion).")
+				end
+			else
+				check is_on_iteration end
+				if attached tag then
+					a_formatter.add ("Loop invariant ")
+					a_formatter.add_manifest_string (tag)
+					a_formatter.add (" might not be maintained.")
+				else
+					a_formatter.add ("Loop invariant might not be maintained (unnamed assertion).")
+				end
+			end
+		end
+
+end
