eve/Src/framework/eiffel2boogie/translation/e2b_attribute_translator.e
@@ -33,6 +33,7 @@ feature -- Basic operations
 			translation_pool.add_type (l_type)
 			l_boogie_name := name_translator.boogie_name_for_feature (a_feature, a_type)
 			create l_constant.make (l_boogie_name, types.field (types.for_type_a (l_type)))
+			l_constant.set_unique
 			boogie_universe.add_declaration (l_constant)
 
 				-- Map attribute slot to original attribute slot
@@ -45,24 +46,25 @@ feature -- Basic operations
 				translation_pool.add_referenced_feature (a_feature, a_feature.written_class.actual_type)
 			end
 
---			if a_feature.type.is_reference then
---				if a_feature.type.is_attached then
---					create l_call.make ("attached_attribute", types.bool)
---				else
---					create l_call.make ("detachable_attribute", types.bool)
---				end
+			if a_feature.type.is_reference then
+				if a_feature.type.is_attached then
+					create l_call.make ("attached_attribute", types.bool)
+				else
+					create l_call.make ("detachable_attribute", types.bool)
+				end
 
---				l_call.add_argument (create {IV_ENTITY}.make ("heap", types.heap_type))
---				l_call.add_argument (create {IV_ENTITY}.make ("o", types.ref))
---				l_call.add_argument (create {IV_ENTITY}.make (l_boogie_name, l_constant.type))
---				l_call.add_argument (factory.type_value (a_feature.type))
+				l_call.add_argument (create {IV_ENTITY}.make ("heap", types.heap_type))
+				l_call.add_argument (create {IV_ENTITY}.make ("o", types.ref))
+				l_call.add_argument (create {IV_ENTITY}.make (l_boogie_name, l_constant.type))
+				l_call.add_argument (factory.type_value (a_feature.type))
 
---				create l_forall.make (l_call)
---				l_forall.add_bound_variable ("heap", types.heap_type)
---				l_forall.add_bound_variable ("o", types.ref)
+				create l_forall.make (l_call)
+				l_forall.add_bound_variable ("heap", types.heap_type)
+				l_forall.add_bound_variable ("o", types.ref)
 
---				create l_axiom.make (l_forall)
---				boogie_universe.add_declaration (l_axiom)
+				create l_axiom.make (l_forall)
+				boogie_universe.add_declaration (l_axiom)
+			end
 --			elseif a_feature.type.is_integer or a_feature.type.is_natural then
 --				create l_heap_access.make ("heap", create {IV_ENTITY}.make ("o", types.ref), create {IV_ENTITY}.make (l_boogie_name, l_constant.type))
 --				create l_call.make ("is_" + a_feature.type.associated_class.name.as_lower, types.bool)
